stuff

src/Tactics.v
@@ -686,3 +686,50 @@ Ltac kinv_or3 :=
     | [H: or3 _ _ _ |- _] => dest_or3; kinv_contra
     end.
 
+
+Section BoolListReflection.
+  Variable A: Type.
+  Variable f: A -> bool.
+
+  Definition evalBoolList ls := fold_left (fun b a => b && f a) ls true.
+
+  Lemma fold_left_true ls: forall v, fold_left (fun b a => b && f a) ls v = true -> v = true.
+  Proof.
+    induction ls; simpl in *; intros; auto.
+    specialize (IHls _ H).
+    destruct v; auto.
+  Qed.
+
+  Lemma fold_left_and_true ls: forall v1 v2,
+                                 fold_left (fun b a => b && f a) ls (v1 && v2) = true ->
+                                 v2 = true /\ fold_left (fun b a => b && f a) ls v1 = true.
+  Proof.
+    induction ls; simpl in *; intros; auto.
+    destruct v1, v2; auto.
+    assert (v1 && v2 && f a = (v1 && f a) && v2) by (destruct v1, v2, (f a); auto).
+    rewrite H0 in H.
+    specialize (IHls _ _ H); dest; auto.
+  Qed.
+
+  Lemma evalBoolList_cons ls: forall a, evalBoolList (a :: ls) = true ->
+                                        f a = true /\ evalBoolList ls = true.
+  Proof.
+    unfold evalBoolList.
+    induction ls; auto; intros; simpl in *.
+    pose proof (fold_left_true _ _ H).
+    apply andb_true_iff in H0; dest.
+    apply fold_left_and_true in H; dest.
+    constructor; auto; subst.
+    rewrite H1.
+    specialize (IHls _ H2); dest.
+    auto.
+  Qed.
+  
+  Lemma boolListReflection ls: evalBoolList ls = true -> forall x, In x ls -> f x = true.
+  Proof.
+    induction ls; simpl in *; auto; intros; simpl in *.
+    apply evalBoolList_cons in H; dest.
+    destruct H0; subst; auto.
+  Qed.
+    
+End BoolListReflection.    
