examples/MemCacheInl.v
@@ -1,0 +1,461 @@
+Require Import Ex.MemCache Lts.Notations Lts.Syntax Lts.Semantics Lts.SemFacts Lts.Refinement.
+Require Import Lts.ParametricEquiv Lts.ParametricInline Lts.ParametricInlineLtac String.
+Require Import Lts.ParametricSyntax.
+
+Theorem traceRefines_trans_elem: forall m1 m2 m3: Modules,
+                                   (m1 <<== m2) -> (m2 <<== m3) -> (m1 <<== m3).
+Proof.
+  intros.
+  unfold MethsT in *; rewrite idElementwiseId in *.
+  eapply traceRefines_trans; eauto.
+Qed.
+
+Section MemCacheInl.
+  Variables IdxBits TagBits LgNumDatas LgDataBytes: nat.
+  Variable Id: Kind.
+
+  Variable FifoSize: nat.
+
+  Open Scope string.
+
+  Require Import Lts.ParametricInlineLtac.
+  Ltac ggNoFilt dm r :=
+    match goal with
+      | mRef:
+          modFromMeta (nmemCache IdxBits TagBits LgNumDatas LgDataBytes Id FifoSize)
+                      <<== modFromMeta ?m,
+          mEquiv: forall ty, MetaModEquiv ty typeUT ?m |- _ =>
+        inlineGenDmGenRule_NoFilt m mEquiv dm r;
+          match goal with
+            | m'Ref:
+                modFromMeta ?m <<== modFromMeta ?m',
+                m'Equiv: forall ty, MetaModEquiv ty typeUT ?m' |- _ =>
+              clear mEquiv;
+                apply (traceRefines_trans_elem mRef) in m'Ref; clear mRef;
+                simpl in m'Ref, m'Equiv; clear m;
+                unfold getGenGenBody, convNameRec, nameVal, nameRec, isRep, projT1
+                  in m'Ref, m'Equiv;
+                repeat autounfold with MethDefs in m'Ref, m'Equiv;
+                rewrite signature_eq in m'Ref, m'Equiv
+          end
+  end.
+
+  Ltac ggFilt dm r :=
+    match goal with
+      | mRef:
+          modFromMeta (nmemCache IdxBits TagBits LgNumDatas LgDataBytes Id FifoSize)
+                      <<== modFromMeta ?m,
+          mEquiv: forall ty, MetaModEquiv ty typeUT ?m |- _ =>
+        inlineGenDmGenRule_Filt m mEquiv dm r;
+          match goal with
+            | m'Ref:
+                modFromMeta ?m <<== modFromMeta ?m',
+                m'Equiv: forall ty, MetaModEquiv ty typeUT ?m' |- _ =>
+              unfold getGenGenBody, convNameRec, nameVal, nameRec, isRep, projT1 in
+                    m'Ref, m'Equiv;
+              repeat autounfold with MethDefs in m'Ref;
+              repeat autounfold with MethDefs in m'Equiv;
+              rewrite signature_eq in m'Ref, m'Equiv;
+              apply (traceRefines_trans_elem mRef) in m'Ref; clear mRef;
+              let newm := fresh in
+              pose m' as newm;
+                fold newm in m'Ref;
+                fold newm in m'Equiv;
+                unfold getGenGenBody, convNameRec, nameVal,
+                       nameRec, isRep, projT1 in newm;
+                repeat autounfold with MethDefs in newm;
+                match type of newm with
+                  | context[SignatureT_dec ?s ?s] =>
+                    rewrite (signature_eq s) in newm; unfold eq_rect in newm
+                end;
+                simpl in newm;
+                clear mEquiv m
+          end
+    end.
+
+  (*
+  (*
+    let dmod := fresh in
+    let dmodRef := fresh in
+    let dmodEquiv := fresh in
+    inlineGenDmGenRule_NoFilt mod modEquiv dm r dmod dmodRef dmodEquiv;
+    changeNames mod modRef modEquiv dmod dmodRef dmodEquiv *)
+
+  Local Notation "'LargeMetaModule'" := {| metaRegs := _;
+                                           metaRules := _;
+                                           metaMeths := _ |}.
+
+
+  
+  Definition nmemCacheInl:
+    {m: MetaModule &
+       (modFromMeta (nmemCache IdxBits TagBits LgNumDatas
+                               LgDataBytes Id FifoSize) <<== modFromMeta m) /\
+        forall ty, MetaModEquiv ty typeUT m}.
+  Proof.
+    pose (nmemCache IdxBits TagBits LgNumDatas LgDataBytes Id FifoSize) as m.
+    assert (mRef: modFromMeta (nmemCache IdxBits TagBits LgNumDatas LgDataBytes Id FifoSize)
+                                <<== modFromMeta m) by
+        (unfold MethsT; rewrite @idElementwiseId; apply traceRefines_refl).
+
+    repeat autounfold with ModuleDefs in m;
+    cbv [makeMetaModule getMetaFromSinNat makeSinModule getMetaFromSin
+                        sinRegs sinRules sinMeths rulesToRep regsToRep methsToRep
+                        convSinToGen] in m;
+    simpl in m;
+    unfold concatMetaMod in m; simpl in m;
+    unfold Indexer.withPrefix in m; simpl in m.
+    assert (mEquiv: forall ty, MetaModEquiv ty typeUT m) by admit.
+
+    
+    Reset Profile.
+    Start Profiling.
+    ggNoFilt "read.cs" "ldHit".
+    Stop Profiling.
+    Show Profile.
+    unfold H in H1, H2.
+    unfold getGenGenBody, convNameRec, nameVal, nameRec, isRep, projT1 in H1, H2.
+    rewrite signature_eq in H2.
+    rewrite signature_eq in H1.
+    clear H.
+    
+
+    Unset Printing Notations.
+    unfold getGenGenBody, convNameRec, nameVal,
+    nameRec, isRep, projT1 in H;
+      repeat autounfold with MethDefs in H.
+    match H with
+      | context[SignatureT_dec ?s ?s] =>
+        rewrite (signature_eq s s) in H;
+          unfold eq_rect in H
+    end.
+      ggNoFilt "read.cs" "stHit".
+    ggNoFilt "read.cs" "l1MissByState".
+    ggNoFilt "read.cs" "l1MissByLine".
+    ggNoFilt "read.cs" "writeback".
+    ggNoFilt "read.cs" "upgRq".
+    ggNoFilt "read.cs" "upgRs".
+    ggNoFilt "read.cs" "ldDeferred".
+    ggNoFilt "read.cs" "stDeferred".
+    ggNoFilt "read.cs" "drop".
+    Stop Profiling.
+    Show Profile.
+    ggFilt "read.cs" "pProcess".
+    ggNoFilt "read.tag" "ldHit".
+    ggNoFilt "read.tag" "stHit".
+    ggNoFilt "read.tag" "l1MissByState".
+    ggNoFilt "read.tag" "l1MissByLine".
+    ggNoFilt "read.tag" "writeback".
+    ggNoFilt "read.tag" "drop".
+
+    let noDupMeth := fresh in
+  let noDupRule := fresh in
+  assert (noDupMeth: NoDup (map getMetaMethName (metaMeths H))) by
+      (subst; simpl; clear; noDup_tac);
+    assert (noDupRule: NoDup (map getMetaRuleName (metaRules H))) by
+      (subst; simpl; clear; noDup_tac);
+    let dmTriple := eval simpl in (findDm "read.tag" nil (metaMeths H)) in
+        let rTriple := eval simpl in (findR "pProcess" nil (metaRules H)) in
+            match dmTriple with
+              | Some (?preDm, @RepMeth ?A ?strA ?goodFn ?GenK ?getConstK
+                                       ?goodFn2 ?bdm ?dmn ?ls ?noDup, ?sufDm) =>
+                match rTriple with
+                  | Some (?preR, @RepRule ?A ?strA ?goodFn ?GenK ?getConstK
+                                          ?goodFn2 ?bdr ?rn ?ls ?noDup, ?sufR) =>
+                    let K1 := fresh in
+                    let K2 := fresh in
+                    let K3 := fresh in
+                    assert
+                      (K1:
+                         forall r',
+                           In r' (preR ++ sufR) ->
+                           match r' with
+                             | OneRule _ _ => true
+                             | RepRule _ _ _ _ _ _ bgenB _ _ _ =>
+                               noCallDmSigGenA (bgenB typeUT)
+                                               {| isRep := true; nameRec := dmn |}
+                                               (projT1 bdm)
+                           end = true) by
+                        (intro;
+                         apply boolListReflection with
+                         (f := (fun r' =>
+                                  match r' with
+                                    | OneRule _ _ => true
+                                    | RepRule _ _ _ _ _ _ bgenB _ _ _ =>
+                                      noCallDmSigGenA (bgenB typeUT)
+                                                      {| isRep := true; nameRec := dmn |}
+                                                      (projT1 bdm)
+                                  end));
+                         repeat
+                           (unfold getGenGenBody, convNameRec, nameVal, nameRec, isRep, projT1;
+                            repeat autounfold with MethDefs;
+                            
+                            repeat match goal with
+                                     | [ |- context[SignatureT_dec ?s ?s] ] =>
+                                       rewrite (signature_eq s); unfold eq_rect
+                                   end; simpl);
+                            apply eq_refl
+                          );
+                      assert
+                        (K2:
+                           forall dm',
+                             In dm' (metaMeths H) ->
+                             match dm' with
+                               | OneMeth _ _ => true
+                               | RepMeth _ _ _ _ _ _ bgenB _ _ _ =>
+                                 noCallDmSigGenA (projT2 bgenB typeUT tt)
+                                                 {| isRep := true; nameRec := dmn |}
+                                                 (projT1 bdm)
+                             end = true) by
+                        (intro;
+                         apply boolListReflection with
+                         (f := (fun dm' =>
+                                  match dm' with
+                                    | OneMeth _ _ => true
+                                    | RepMeth _ _ _ _ _ _ bgenB _ _ _ =>
+                                      noCallDmSigGenA (projT2 bgenB typeUT tt)
+                                                      {| isRep := true; nameRec := dmn |}
+                                                      (projT1 bdm)
+                                  end)); apply eq_refl);
+                      assert
+                        (K3: exists call : NameRecIdx,
+                               In call (getCallsGenA (bdr typeUT)) /\
+                               nameVal (nameRec call) = nameVal dmn /\ isRep call = true)
+                        by
+                          (eexists {| isRep := true;
+                                      nameRec := {| nameVal := nameVal dmn;
+                                                    goodName := _ |} |};
+                           split; [
+                             
+                             repeat (unfold getGenGenBody, convNameRec, nameVal, nameRec, isRep, projT1;
+                             repeat autounfold with MethDefs;
+                             
+                             repeat match goal with
+                                      | [ |- context[SignatureT_dec ?s ?s] ] =>
+                                        rewrite (signature_eq s); unfold eq_rect
+                                    end; simpl)
+                             ; tauto | split; reflexivity]);
+                      pose proof (@inlineGenGenDmToRule_traceRefines_Filt'
+                                    H H5 A strA goodFn GenK getConstK goodFn2
+                                    bdm dmn preDm sufDm ls noDup eq_refl bdr rn preR
+                                    sufR eq_refl noDupMeth noDupRule K1 K2 K3);
+                        pose proof (@inlineGenGenDmToRule_ModEquiv_Filt'
+                                      H H5 A strA goodFn GenK getConstK goodFn2
+                                      bdm dmn preDm sufDm ls noDup eq_refl bdr rn preR
+                                      sufR eq_refl noDupMeth noDupRule K2);
+                        clear noDupMeth noDupRule K1 K2 K3
+                end
+            end.
+    eexists {| isRep := true;
+               nameRec := {| nameVal := "read.tag";
+                             goodName := _ |} |}.
+    split; [| split; reflexivity].
+    unfold getGenGenBody, convNameRec, nameVal, nameRec, isRep, projT1;
+      repeat autounfold with MethDefs;
+      
+      repeat match goal with
+               | [ |- context[SignatureT_dec ?s ?s] ] =>
+                 rewrite (signature_eq s); unfold eq_rect
+             end; simpl. tauto.
+    unfold getGenGenBody, convNameRec.    simpl.
+    simpl.
+    intro;
+      eapply boolListReflection with
+      (f := (fun r' =>
+               match r' with
+                 | OneRule _ _ => true
+                 | RepRule _ _ _ _ _ _ bgenB _ _ _ =>
+                   noCallDmSigGenA (bgenB typeUT)
+                                   {| isRep := true; nameRec := _ |}
+                                   (projT1 _)
+               end)).
+    repeat (unfold getGenGenBody, convNameRec, nameVal, nameRec, isRep, projT1;
+      repeat autounfold with MethDefs;
+      repeat match goal with
+               | [ |- context[SignatureT_dec ?s ?s] ] =>
+                 rewrite (signature_eq s); unfold eq_rect
+             end; simpl);
+      reflexivity.
+
+    eexists {| isRep := true;
+               nameRec := {| nameVal := nameVal _;
+                             goodName := _ |} |}.
+      split; [simpl; tauto | split; reflexivity]
+               apply eq_refl.
+                         
+    
+    inlineGenDmGenRule_Filt H H5 "read.tag" "pProcess".
+
+    ggFilt "read.tag" "pProcess".
+    ggNoFilt "read.line" "ldHit".
+    ggNoFilt "read.line" "stHit".
+    ggNoFilt "read.cs" "writeback".
+    ggNoFilt "read.cs" "ldDeferred".
+    ggNoFilt "read.cs" "stDeferred".
+    ggFilt "read.cs" "pProcess".
+
+    Stop Profiling.
+    Show Profile.
+
+inlineGenDmGenRule_Filt H0 H5 "read.cs" "pProcess".
+intro.
+apply boolListReflection with (f := (fun dm' =>
+                                       match dm' with
+                                         | OneMeth _ _ => true
+                                         | RepMeth _ _ _ _ _ _ bgenB _ _ _ =>
+                                           noCallDmSigGenA (projT2 bgenB typeUT tt)
+                                                           {| isRep := true; nameRec := dmn |}
+                                                           (projT1 bdm)
+                                       end)).
+                                     .
+clear; intros; dest_in; simpl.
+unfold getGenGenBody, convNameRec, nameVal, nameRec, isRep, projT1;
+  repeat autounfold with MethDefs.
+match goal with
+  | [ |- context[SignatureT_dec ?s ?s] ] =>
+    rewrite (signature_eq s); unfold eq_rect
+end.
+reflexivity.
+
+unfold getGenGenBody.
+unfold convNameRec.
+unfold nameVal.
+unfold nameRec.
+unfold isRep.
+unfold projT1.
+unfold StringEq.string_eq.
+reflexivity.
+    let isIn := fresh in
+    clear; intros ? isIn;
+    repeat (destruct isIn as [? | isIn]; [subst; reflexivity | ]);
+    exfalso; apply isIn.
+               destruct isIn.
+    
+                        (*(let isIn := fresh in
+                         intros ? ? ? ? ? ? ? ? ? ? isIn;
+                         repeat (destruct isIn as [? | isIn]; [subst; reflexivity | ]);
+                         destruct isIn); *)
+
+    
+    intros ? ? ? ? ? ? ? ? ? ? isIn; simpl in isIn.
+    destruct isIn as [murali | isIn].
+    
+    inversion murali.
+    injection murali as [_ _ _ _ bgen _ _].
+    inversion murali; subst; clear murali.
+    simpl.
+    inv murali.
+    [subst; reflexivity | ].
+    repeat (destruct isIn as [? | isIn]; [subst; reflexivity | ]).
+    repeat (destruct isIn as [? | isIn]; [subst; reflexivity | ]).
+    destruct isIn.
+                    asser
+    clear m.
+    match goal with
+      | m'Ref:
+          modFromMeta _ <<== modFromMeta ?m',
+          m'Equiv: forall ty, MetaModEquiv ty typeUT ?m' |- _ =>
+        let newm := fresh in
+        pose m' as newm;
+          fold newm in m'Ref;
+          fold newm in m'Equiv;
+          simpl in newm;
+          clear m
+    end.
+    clear m.
+    inlineGenDmGenRule_NoFilt m mEquiv "read.cs" "ldHit".
+    Reset Profile.
+    Start Profiling.
+
+    let noDupMeth := fresh in
+  let noDupRule := fresh in
+  assert (noDupMeth: NoDup (map getMetaMethName (metaMeths m))) by
+    (subst; simpl; clear; noDup_tac);
+    assert (noDupRule: NoDup (map getMetaRuleName (metaRules m))) by
+      (subst; simpl; clear; noDup_tac);
+    let dmTriple := eval simpl in (findDm "read.cs" nil (metaMeths m)) in
+        let rTriple := eval simpl in (findR "ldHit" nil (metaRules m)) in
+            match dmTriple with
+              | Some (?preDm, @RepMeth ?A ?strA ?goodFn ?GenK ?getConstK
+                                       ?goodFn2 ?bdm ?dmn ?ls ?noDup, ?sufDm) =>
+                match rTriple with
+                  | Some (?preR, @RepRule ?A ?strA ?goodFn ?GenK ?getConstK
+                                          ?goodFn2 ?bdr ?rn ?ls ?noDup, ?sufR) =>
+                    let m'Ref := fresh in
+                    let m'Equiv := fresh in
+                    pose proof (@inlineGenGenDmToRule_traceRefines_NoFilt
+                                  m A strA goodFn GenK getConstK goodFn2
+                                  bdm dmn preDm sufDm ls noDup eq_refl bdr rn preR
+                                  sufR eq_refl noDupMeth noDupRule) as m'Ref;
+                      pose proof (@inlineGenGenDmToRule_ModEquiv_NoFilt
+                                    m mEquiv A strA goodFn GenK getConstK goodFn2
+                                    bdm dmn preDm sufDm ls noDup eq_refl bdr rn preR
+                                    sufR eq_refl noDupMeth noDupRule) as m'Equiv;
+                      clear noDupMeth noDupRule
+                end
+            end.
+
+    
+    inlineGenDmGenRule_NoFilt m mEquiv "read.cs" "ldHit".
+    match goal with
+      | mRef:
+          modFromMeta (nmemCache IdxBits TagBits LgNumDatas LgDataBytes Id FifoSize)
+                      <<== modFromMeta ?m,
+          mEquiv: forall ty, MetaModEquiv ty typeUT ?m |- _ =>
+        inlineGenDmGenRule_NoFilt m mEquiv dm r;
+          match goal with
+            | m'Ref:
+                modFromMeta ?m <<== modFromMeta ?m',
+              m'Equiv: forall ty, MetaModEquiv ty typeUT ?m' |- _ =>
+              pose proof (traceRefines_trans_elem mRef m'Ref); clear mRef m'Ref;
+              pose m' as newm;
+              fold newm in m'Ref;
+              fold newm in m'Equiv;
+              clear m
+          end;
+          clear mEquiv
+    end.
+    
+    ggNoFilt "read.cs" "ldHit".
+
+    ggNoFilt "read.cs" "stHit".
+
+
+    ggNoFilt "read.cs" "upgRq".
+
+    Stop Profiling.
+    Show Profile.
+
+    Reset Profile.
+    Start Profiling.
+    ggNoFilt "read.cs" "upgRs".
+    Stop Profiling.
+    Show Profile.
+
+
+    ggNoFilt "read.cs" "l1MissByState".
+
+    Stop Profiling.
+    Show Profile.
+
+    Reset Profile.
+    Start Profiling.
+    
+    ggNoFilt mod modRef modEquiv "read.cs" "l1MissByLine".
+    Stop Profiling.
+    Show Profile.
+    
+    ggNoFilt mod modRef modEquiv "read.cs" "ldDeferred".
+    ggNoFilt mod modRef modEquiv "read.cs" "stDeferred".
+    ggNoFilt mod modRef modEquiv "read.cs" "drop".
+    ggNoFilt mod modRef modEquiv "read.cs" "writeback".
+    ggFilt mod modRef modEquiv "read.cs" "pProcess".
+    
+    exact (existT _ mod (conj modRef modEquiv)).
+    admit.
+  Defined.
+
+  Close Scope string.
+
+  *)
+End MemCacheInl.
