src/ParametricInlineLtac.v
@@ -1,4 +1,4 @@
-Require Import ParametricInline List ParametricSyntax String Syntax CommonTactics.
+Require Import ParametricInline List ParametricSyntax String Syntax Lib.CommonTactics Tactics.
 
 Fixpoint findDm dm pre ls :=
   match ls with
@@ -54,8 +54,6 @@ Fixpoint findR dm pre ls :=
       end
   end.
 
-Local  Notation "'LargeMetaModule'" := {| metaRegs := _; metaRules := _; metaMeths := _ |}.
-
 Ltac inlineGenDmGenRule_NoFilt m mEquiv dm r (*dmod dmodRef dmodEquiv*) :=
   let noDupMeth := fresh in
   let noDupRule := fresh in
@@ -76,35 +74,96 @@ Ltac inlineGenDmGenRule_NoFilt m mEquiv dm r (*dmod dmodRef dmodEquiv*) :=
                     pose proof (@inlineGenGenDmToRule_traceRefines_NoFilt
                                   m A strA goodFn GenK getConstK goodFn2
                                   bdm dmn preDm sufDm ls noDup eq_refl bdr rn preR
-                                  sufR eq_refl noDupMeth noDupRule) as m'Ref;
+                                  sufR eq_refl noDupMeth noDupRule);
                       pose proof (@inlineGenGenDmToRule_ModEquiv_NoFilt
                                     m mEquiv A strA goodFn GenK getConstK goodFn2
                                     bdm dmn preDm sufDm ls noDup eq_refl bdr rn preR
-                                    sufR eq_refl noDupMeth noDupRule) as m'Equiv;
-                    (*
-                    pose {| metaRegs := metaRegs m;
-                            metaRules :=
-                              preR ++ RepRule strA goodFn getConstK goodFn2
-                                   (fun ty => inlineGenGenDm (bdr ty) dm bdm)
-                                   rn noDup :: sufR;
-                            metaMeths := metaMeths m |} as dmod;
-                      pose proof
-                           (@inlineGenGenDmToRule_traceRefines_NoFilt
-                              m A strA goodFn GenK getConstK goodFn2
-                              bdm dmn preDm sufDm ls noDup eq_refl bdr rn preR
-                              sufR eq_refl noDupMeth noDupRule) as dmodRef;
-                      replace LargeMetaModule with dmod in dmodRef by reflexivity;
-                      pose proof
-                           (@inlineGenGenDmToRule_ModEquiv_NoFilt
-                              m mEquiv A strA goodFn GenK getConstK goodFn2
-                              bdm dmn preDm sufDm ls noDup eq_refl bdr rn preR
-                              sufR eq_refl noDupMeth noDupRule) as dmodEquiv;
-                      replace LargeMetaModule with dmod in dmodEquiv by reflexivity;
-                     *)
+                                    sufR eq_refl noDupMeth noDupRule);
                       clear noDupMeth noDupRule
                 end
             end.
 
+Ltac inlineGenDmGenRule_Filt m mEquiv dm r :=
+  let noDupMeth := fresh in
+  let noDupRule := fresh in
+  assert (noDupMeth: NoDup (map getMetaMethName (metaMeths m))) by
+      (subst; simpl; clear; noDup_tac);
+    assert (noDupRule: NoDup (map getMetaRuleName (metaRules m))) by
+      (subst; simpl; clear; noDup_tac);
+    let dmTriple := eval simpl in (findDm dm nil (metaMeths m)) in
+        let rTriple := eval simpl in (findR r nil (metaRules m)) in
+            match dmTriple with
+              | Some (?preDm, @RepMeth ?A ?strA ?goodFn ?GenK ?getConstK
+                                       ?goodFn2 ?bdm ?dmn ?ls ?noDup, ?sufDm) =>
+                match rTriple with
+                  | Some (?preR, @RepRule ?A ?strA ?goodFn ?GenK ?getConstK
+                                          ?goodFn2 ?bdr ?rn ?ls ?noDup, ?sufR) =>
+                    let H3 := fresh in
+                    let H4 := fresh in
+                    let H5 := fresh in
+                    assert
+                      (H3:
+                         forall r',
+                           In r' (preR ++ sufR) ->
+                           match r' with
+                             | OneRule _ _ => true
+                             | RepRule _ _ _ _ _ _ bgenB _ _ _ =>
+                               noCallDmSigGenA (bgenB typeUT)
+                                               {| isRep := true; nameRec := dmn |}
+                                               (projT1 bdm)
+                           end = true) by
+                        (intro;
+                         apply boolListReflection with
+                         (f := (fun r' =>
+                                  match r' with
+                                    | OneRule _ _ => true
+                                    | RepRule _ _ _ _ _ _ bgenB _ _ _ =>
+                                      noCallDmSigGenA (bgenB typeUT)
+                                                      {| isRep := true; nameRec := dmn |}
+                                                      (projT1 bdm)
+                                  end)); apply eq_refl);
+                      assert
+                        (H4:
+                           forall dm',
+                             In dm' (metaMeths m) ->
+                             match dm' with
+                               | OneMeth _ _ => true
+                               | RepMeth _ _ _ _ _ _ bgenB _ _ _ =>
+                                 noCallDmSigGenA (projT2 bgenB typeUT tt)
+                                                 {| isRep := true; nameRec := dmn |}
+                                                 (projT1 bdm)
+                             end = true) by
+                        (intro;
+                         apply boolListReflection with
+                         (f := (fun dm' =>
+                                  match dm' with
+                                    | OneMeth _ _ => true
+                                    | RepMeth _ _ _ _ _ _ bgenB _ _ _ =>
+                                      noCallDmSigGenA (projT2 bgenB typeUT tt)
+                                                      {| isRep := true; nameRec := dmn |}
+                                                      (projT1 bdm)
+                                  end)); apply eq_refl);
+                      assert
+                        (H5: exists call : NameRecIdx,
+                               In call (getCallsGenA (bdr typeUT)) /\
+                               nameVal (nameRec call) = nameVal dmn /\ isRep call = true) by
+                          (eexists {| isRep := true;
+                                      nameRec := {| nameVal := nameVal dmn;
+                                                    goodName := _ |} |};
+                           split; [
+                             simpl; tauto | split; reflexivity]);
+                      pose proof (@inlineGenGenDmToRule_traceRefines_Filt'
+                                    m mEquiv A strA goodFn GenK getConstK goodFn2
+                                    bdm dmn preDm sufDm ls noDup eq_refl bdr rn preR
+                                    sufR eq_refl noDupMeth noDupRule H3 H4 H5);
+                        pose proof (@inlineGenGenDmToRule_ModEquiv_Filt'
+                                      m mEquiv A strA goodFn GenK getConstK goodFn2
+                                      bdm dmn preDm sufDm ls noDup eq_refl bdr rn preR
+                                      sufR eq_refl noDupMeth noDupRule H4);
+                        clear noDupMeth noDupRule H3 H4 H5
+                end
+            end.
+(*
 Ltac inlineGenDmGenRule_Filt m mEquiv dm r :=
   let noDupMeth := fresh in
   let noDupRule := fresh in
@@ -187,6 +246,7 @@ Ltac inlineGenDmGenRule_Filt m mEquiv dm r :=
                         clear noDupMeth noDupRule H3 H4 H5
                 end
             end.
+*)
 
 Ltac inlineSinDmGenRule_Filt m mEquiv dm r :=
   let dmTriple := eval simpl in (findDm dm nil (metaMeths m)) in
